\documentclass{ximera}

\input{../preamble.tex}

\title[Dig-In:]{Horizontal asymptotes}

\outcome{Find horizontal asymptotes using limits.}
\outcome{Recognize that a curve can cross a horizontal asymptote.}
\outcome{Calculate the limit as $x$ approaches $\pm \infty$ of common functions algebraically.}
\outcome{Find the limit as $x$ approaches $\pm \infty$ from a graph.}
\outcome{Define a horizontal asymptote.}
\outcome{Compute limits at infinity of famous functions.}
\outcome{Identify horizontal asymptotes by looking at a graph.}

\begin{document}
\begin{abstract}
We explore functions that behave like horizontal lines as the input
grows without bound.
\end{abstract}
\maketitle



Consider the function:
\[
f(x) = \frac{6x-9}{x-1}
\]
\begin{image}
\begin{tikzpicture}
	\begin{axis}[
            domain=1:4,
            ymax=20,
            ymin=-10,
            samples=100,
            axis lines =middle, xlabel=$x$, ylabel=$y$,
            every axis y label/.style={at=(current axis.above origin),anchor=south},
            every axis x label/.style={at=(current axis.right of origin),anchor=west}
          ]
	  \addplot [very thick, penColor, smooth, domain=(0:.9)] {(6*x-9)/(x-1)};
          \addplot [very thick, penColor, smooth, domain=(1.1:3)] {(6*x-9)/(x-1)};
          \addplot [textColor, dashed] plot coordinates {(1,-10) (1,20)};
        \end{axis}
\end{tikzpicture}
%% \caption{A plot of $f(x)=\protect\frac{6x-9}{x-1}$.}
%% \label{plot:(6x-9)/(x-1)}
\end{image}
As $x$ approaches infinity, it seems like $f(x)$ approaches a specific
value. Such a limit is called a \textit{limit at infinity}.


%%DEFINITIONS
\begin{definition}\label{def:limitAtInfty}\index{limit!at infinity}
If $f(x)$ becomes arbitrarily close to a specific value $L$ by making
$x$ sufficiently large, we write
\[
\lim_{x\to \infty} f(x) = L
\]
and we say, the \dfn{limit at infinity} of $f(x)$ is $L$.  

If $f(x)$ becomes arbitrarily close to a specific value $L$ by making
$x$ sufficiently large and negative, we write
\[
\lim_{x\to -\infty} f(x) = L
\]
and we say, the \dfn{limit at negative infinity} of $f(x)$ is $L$.  
\end{definition}

%%Example 1
\begin{example} Compute
\[
\lim_{x\to\infty} \frac{6x-9}{x-1}.
\]
\begin{explanation}
Write
\begin{align*}
\lim_{x\to\infty}\frac{6x-9}{x-1} &= \lim_{x\to\infty}\frac{6x-9}{x-1}\cdot \frac{1/x}{1/x}\\
&=\lim_{x\to\infty}\frac{\frac{6x}{x} - \frac{9}{x}}{\frac{x}{x} - \frac{1}{x}}\\
&= \lim_{x\to\infty} \frac{6}{1}\\
&= 6.
\end{align*}
\end{explanation}
\end{example}

%%Example 2
\begin{example} Compute
\[
\lim_{x\to\infty} \frac{6x-9}{x^2-1}.
\]
\begin{explanation}
Write
\begin{align*}
\lim_{x\to\infty}\frac{6x-9}{x^2-1} &= \lim_{x\to\infty}\frac{6x-9}{x^2-1}\cdot \frac{1/x^2}{1/x^2}\\
&=\lim_{x\to\infty}\frac{\frac{6x}{x^2} - \frac{9}{x^2}}{\frac{x}{x^2} - \frac{1}{x^2}}\\
&= \lim_{x\to\infty} \frac{\frac{6}{x}-\frac{9}{x^2}}{1-\frac{1}{x^2}}\\
&= \frac{0}{1}=0.
\end{align*}
\end{explanation}
\end{example}

%%CONSIDER 1/X
Notice that in both examples, the numerator and denominator are multiplied by $\displaystyle\frac{1}{\phantom{xx}x^{\text{highest power in denominator}}\phantom{xx}}$.

Why is this the case? Let's consider the basic rational function

\[
f(x) = \frac{1}{x}
\]
\begin{image}
\begin{tikzpicture}
	\begin{axis}[
            domain=-4:4,
            ymax=20,
            ymin=-10,
            samples=100,
            axis lines =middle, xlabel=$x$, ylabel=$y$,
            every axis y label/.style={at=(current axis.above origin),anchor=south},
            every axis x label/.style={at=(current axis.right of origin),anchor=west}
          ]
	  \addplot [very thick, penColor, smooth, domain=(-3:-0.01)] {(1)/(x)};
      \addplot [very thick, penColor, smooth, domain=(0.01:3)] {(1)/(x)};
      \addplot [textColor, dashed] plot coordinates {(0,-20) (0,20)};
 
          
        \end{axis}
\end{tikzpicture}
\end{image}
As $x$ approaches infinity, $f(x)$ approaches $0$. If we can get individual terms in our rational function to ``look like'' the known basic rational function $f(x)=\frac{1}{x}$, then we can more easily evaluate the limit as $x$ approaches infinity. Therefore, the technique applied to $\displaystyle\lim_{x\to \infty}\frac{numerator}{denominator}$ is to multiply the numerator and denominator by $\displaystyle\frac{1}{\phantom{xx}x^{\text{highest power in denominator}}\phantom{xx}}$.


%%Example 3
\begin{example} Compute
\[
\lim_{x\to\infty} \frac{3x^4-5x^2+1}{x^2-x+2x^4}.
\]
\begin{explanation}
Write
\begin{align*}
\lim_{x\to\infty}\frac{3x^4-5x^2+1}{x^2-x+2x^4} &= \lim_{x\to\infty}\frac{3x^4-5x^2+1}{x^2-x+2x^4}\cdot \frac{1/x^4}{1/x^4}\\
&=\lim_{x\to\infty}\frac{\frac{3x^4}{x^4} - \frac{5x^2}{x^4}+\frac{1}{x^4}}{\frac{x^2}{x^4}-\frac{x}{x^4} + \frac{2x^4}{x^4}}\\
&= \lim_{x\to\infty} \frac{3-\frac{5}{x^2}+\frac{1}{x^4}}{\frac{1}{x^2}-\frac{1}{x^3}+2}\\
&= \frac{3}{2}.
\end{align*}
\end{explanation}
\end{example}

Sometimes one must be careful, consider this example.

\begin{example}
Compute
\[
\lim_{x\to -\infty} \frac{x^3+1}{\sqrt{x^6+5}}
\]
\begin{explanation}
In this case we multiply the numerator and denominator by $-1/x^3$,
which is a positive number as since $x\to -\infty$, $x^3$ is a negative
number.
\begin{align*}
\lim_{x\to -\infty} \frac{x^3+1}{\sqrt{x^6+5}} &= \lim_{x\to -\infty} \frac{x^3+1}{\sqrt{x^6+5}} \cdot \frac{-1/x^3}{-1/x^3}\\
&= \lim_{x\to -\infty} \frac{-1-1/x^3}{\sqrt{x^6/x^6+5/x^6}}\\
&= -1.
\end{align*}
\end{explanation}
\end{example}

Note, since
\[
\lim_{x\to \infty} f(x) = \lim_{x\to 0^+} f\left(\frac{1}{x}\right)
\]
and
\[
\lim_{x\to -\infty} f(x) = \lim_{x\to 0^-} f\left(\frac{1}{x}\right)
\]
we can also apply the Squeeze Theorem when taking limits at infinity.
Here is an example of a limit at infinity that uses the Squeeze
Theorem, and shows that functions can, in fact, cross their horizontal
asymptotes.


\begin{example}
Compute:
\[
\lim_{x\to \infty} \frac{\sin(7x)+4x}{x}
\]
\begin{image}
\begin{tikzpicture}
	\begin{axis}[
            domain=2:20,
            ymax=5,
            ymin=3,
            samples=100,
            axis lines =middle, xlabel=$x$, ylabel=$y$,
            every axis y label/.style={at=(current axis.above origin),anchor=south},
            every axis x label/.style={at=(current axis.right of origin),anchor=west}
          ]
	  \addplot [very thick, penColor, smooth] {(1/x) * sin(deg(7*x))+4};
        \end{axis}
\end{tikzpicture}
%% \caption{A plot of $f(x)=\frac{\sin(7x)}{x}+4$.}
%% \label{plot:sin7x/x+4}
\end{image}

\begin{explanation}
We can bound our function
\[
\frac{-1+4x}{x} \le \frac{\sin(7x)+4x}{x} \le \frac{1+4x}{x}.
\]
Now write with me
\begin{align*}
\displaystyle\lim_{x\to\infty}\frac{-1+4x}{x} \cdot \frac{1/x}{1/x} &= \lim_{x\to\infty}\frac{-1/x+4}{1}\\
&=4.
\end{align*}
And we also have
\begin{align*}
\displaystyle\lim_{x\to\infty}\frac{1+4x}{x} \cdot \frac{1/x}{1/x} &= \lim_{x\to\infty}\frac{1/x+4}{1}\\
&=4.
\end{align*}
Since 
\[
\lim_{x\to \infty} \frac{-1+4x}{x}  = 4 = \lim_{x\to \infty}\frac{1+4x}{x} 
\] 
we conclude by the Squeeze Theorem,
$\displaystyle\lim_{x\to\infty}\frac{\sin(7x)}{x}+4 = 4$.
\end{explanation}
\end{example}






\begin{definition}\label{def:horiz asymptote}\index{asymptote!horizontal}\index{horizontal asymptote}
If  
\[
\lim_{x\to \infty} f(x) = L \qquad\text{or}\qquad \lim_{x\to -\infty} f(x) = L,
\]
then the line $y=L$ is a \dfn{horizontal asymptote} of $f(x)$.
\end{definition}

\begin{example} 
Give the horizontal asymptotes of
\[
f(x) = \frac{6x-9}{x-1}
\]
\begin{explanation}
From our previous work, we see that $\displaystyle\lim_{x\to \infty} f(x) = 6$, and
upon further inspection, we see that $\displaystyle\lim_{x\to -\infty} f(x) =
6$. Hence the horizontal asymptote of $f(x)$ is the line $y=6$.
\end{explanation}
\end{example}


It is a common misconception that a function cannot cross an
asymptote. As the next example shows, a function can cross a horizontal
asymptote, and in the example this occurs an infinite number of times!

\begin{example}
Give a horizontal asymptote of
\[
f(x) = \frac{\sin(7x)+4x}{x}.
\]
\begin{explanation}
Again from previous work, we see that $\displaystyle\lim_{x\to \infty} f(x) =
\answer[given]{4}$. Hence $y=\answer[given]{4}$ is a horizontal asymptote of $f(x)$.
\end{explanation}
\end{example}




\end{document}
