\documentclass{ximera}


\outcome{Calculate limits using the limit laws.}

\input{../preamble.tex}
\title[Dig-In:]{The limit laws}
\begin{document}
\begin{abstract}
We give basic laws for working with limits. 
\end{abstract}
\maketitle

In this section, we present a handful of rules called the \textit{Limit Laws}
that allow us to find limits of various combinations of functions.

\begin{theorem}[Limit Laws]\index{limit laws}\label{theorem:limit-laws}
Suppose that $\displaystyle\lim_{x\to a}f(x)=L$, $\displaystyle\lim_{x\to a}g(x)=M$.
\begin{description}
\item[\textbf{Constant Multiple Law}] $\displaystyle\lim_{x\to a} kf(x) = k\displaystyle\lim_{x\to a}f(x)=kL$.\\
\item[Sum/Difference Law] $\displaystyle\lim_{x\to a} (f(x) \pm g(x)) =
  \lim_{x\to a}f(x) \pm \lim_{x\to a}g(x)=L \pm M$.
\item[Product Law]  $\displaystyle\lim_{x\to a} (f(x)g(x)) = \displaystyle\lim_{x\to
  a}f(x)\cdot\lim_{x\to a}g(x)=LM$.
\item[Quotient Law]  $\displaystyle\lim_{x\to a} \frac{f(x)}{g(x)} =
  \frac{\displaystyle\lim_{x\to a}f(x)}{\displaystyle\lim_{x\to a}g(x)}=\frac{L}{M}$, if
  $M\ne0$.
\end{description}
\label{thm:limit laws}
\end{theorem}


\begin{example}
  Compute the following limit using limit laws:
  \[
  \displaystyle\lim_{x\to 1}(5x^2+3x-2)
  \]
\begin{explanation}
  Well, get out your pencil and write with me:
  \[
  \displaystyle\lim_{x\to 1} (5x^2+3x-2) = \lim_{x\to 1} 5x^2 + \lim_{x\to 1} \answer[given]{3x} - \lim_{x\to 1}2
  \]
  by the Sum/Difference Law. So now
  \[
  = 5\displaystyle\lim_{x\to 1} x^2 + 3\lim_{x\to 1} x - \lim_{x\to 1}\answer[given]{2}
  \]
  
  \[
  = 5(1)^2 + 3(1) - 2 =\answer[given]{6}.
  \]
  \begin{prompt}
    We can check our answer by looking at the graph of $y=f(x)$:
    \[
    \graph{5x^2+3x-2}
    \]
  \end{prompt}
\end{explanation}  
\end{example}


The most important thing to learn from this section is whether the
limit laws can be applied for a certain problem, and when we need to
do something more interesting.  We will begin discussing those more
interesting cases in the next section.  For now, we end this section
with a question:

\section{A list of questions}

Let's try this out.

\begin{question}
  Can this limit be directly computed by limit laws?
  \[
  \displaystyle\lim_{x\to 2}\frac{x^2+3x+2}{x+2} 
  \]
  \begin{multipleChoice}
    \choice[correct]{yes}
    \choice{no}
  \end{multipleChoice}
  \begin{question}
    Compute:
    \[
    \displaystyle\lim_{x\to 2}\frac{x^2+3x+2}{x+2}\begin{prompt} =\answer{3}\end{prompt}
    \]
    \begin{feedback}
      Since $f(x)=\frac{x^2+3x+2}{x+2}$ is a rational function, and
      the denominator does not equal $0$, we see that $f(x)$ is
      continuous at $x=2$.  Thus, to find this limit, it suffices to
      plug $2$ into $f(x)$.
    \end{feedback}
  \end{question}
\end{question}


\begin{question}
  Can this limit be directly computed by limit laws?
  \[
  \displaystyle\lim_{x\to 2}\frac{x^2-3x+2}{x-2}
  \]
  \begin{multipleChoice}
    \choice{yes}
    \choice[correct]{no}
  \end{multipleChoice}
  \begin{feedback}
    $f(x) = \frac{x^2-3x+2}{x-2}$ is a rational function, but the
    denominator $x-2$ equals $0$ when $x=2$. None of our current
    theorems address the situation when the denominator of a fraction
    approaches $0$.
  \end{feedback}
\end{question}


\begin{question}
  Can this limit be directly computed by limit laws?
  \[
  \displaystyle\lim_{x\to 0} x\sin(1/x)
  \]
  \begin{multipleChoice}
    \choice{yes}
    \choice[correct]{no}
  \end{multipleChoice}
  \begin{feedback}
    If we are trying to use limit laws to compute this limit, we would
    first have to use the Product Law to say that
    \[
    \displaystyle\lim_{x\to 0}x\sin(1/x)= \lim_{x\to 0} x \cdot \lim_{x\to 0} \sin(1/x).
    \]
    We are only allowed to use this law if both limits exist, so we
    must check this first.  We know from continuity that
    \[
    \displaystyle\lim_{x\to  0}x=0.
    \]
    However, we also know that $\sin(1/x)$ oscillates ``wildly'' as
    $x$ approaches $0$, and so the limit
    \[
    \lim_{x\to 0} \sin(1/x)
    \]does not exist.  Therefore, we cannot use the
    Product Law.
  \end{feedback}
\end{question}


\begin{question}
  Can this limit be directly computed by limit laws?
  \[
  \displaystyle\lim_{x\to 0} \cot(x^3)
  \]
  \begin{multipleChoice}
    \choice{yes}
    \choice[correct]{no}
  \end{multipleChoice}
  \begin{feedback}
    Notice that
    \[
    \cot(x^3) = \frac{\cos(x^3)}{\sin(x^3)}.
    \]
    If we are trying to use limit laws to compute this limit, we would
    like to use the Quotient Law to say that
    \[
    \displaystyle\lim_{x\to 0} \frac{\cos(x^3)}{\sin(x^3)} = \displaystyle\frac{\lim_{x\to 0}
      \cos(x^3)}{\lim_{x\to 0} \sin(x^3)}.
    \]
    We are only allowed to use this law if both limits exist and the
    denominator is not $0$. We suspect that the limit on on the
    denominator might equal $0$, so we check this limit.
    \begin{align*}
      \displaystyle\lim_{x\to 0} \sin(x^3) &= \displaystyle\sin(\lim_{x\to 0}x^3)\\
      &=\sin(0) \\
      &=0.
  \end{align*}
  This means that the denominator is zero and hence we cannot use the
  Quotient Law.
  \end{feedback}
\end{question}


\begin{question}
  Can this limit be directly computed by limit laws?
  \[
  \displaystyle\lim_{x\to 1}\sec^2(\sqrt{x}-1)
  \]
  \begin{multipleChoice}
    \choice[correct]{yes}
    \choice{no}
  \end{multipleChoice}
  \begin{question}
    Compute:
    \[
    \displaystyle\lim_{x\to 1}\sec^2(\sqrt{x}-1)\begin{prompt} =\answer{1}\end{prompt}
    \]
    \begin{feedback}
      Notice that
      \[
      \displaystyle\lim_{x\to 1} \sec^2(\sqrt{x}-1) = \lim_{x\to 1} \frac{1}{\cos^2(\sqrt{x}-1)}.
      \]
      If we are trying to use Limit Laws to compute this limit, we
      would now have to use the Quotient Law to say that
      \[
      \displaystyle\lim_{x\to 1} \frac{1}{\cos^2(\sqrt{x}-1)} = \frac{ \lim_{x\to 1}1}{
        \lim_{x\to 1}\cos^2(\sqrt{x}-1)}.
      \]
      We are only allowed to use this law if both limits exist and the
      denominator is not $0$.  Let's check the denominator and numerator
      separately. First we'll compute the limit of the denominator:
      \begin{align*}
        \displaystyle\lim_{x\to 1}\cos^2(\sqrt{x}-1) &= \cos^2(\lim_{x\to 1}(\sqrt{x}-1))\\
        &=\cos^2(\lim_{x\to 1}(\sqrt{x})-\lim_{x\to 1}(1))\\
        &=\cos^2(1-1)\\
        &= \cos^2(0)\\
        &=1
      \end{align*}
      Therefore, the limit in the denominator exists and does not
      equal $0$. We can use the Quotient Law, so we will compute the limit of the numerator:
      \[
      \lim_{x\to 1}1=1
      \]
      Hence
      \[
      \frac{ \lim_{x\to 1}1}{ \lim_{x\to 1}\cos^2(\sqrt{x}-1)} =
      \frac{1}{1}=1
      \]
    \end{feedback}
  \end{question}
\end{question}


\begin{question}
  Can this limit be directly computed by limit laws?
  \[
  \displaystyle\lim_{x\to 4}{\left(\frac{2x}{x-4}-\frac{8}{x-4}\right)}
  \]
  \begin{multipleChoice}
    \choice{yes}
    \choice[correct]{no}
  \end{multipleChoice}
  \begin{feedback}
    If we are trying to use limit laws to compute this limit, we would have to use the Product Law to say that
    \[
    \displaystyle\lim_{x\to 4}\left(\frac{2x}{x-4} - \frac{8}{x-4}\right)= \displaystyle\lim_{x\to 4}\frac{2x}{x-4} - \lim_{x\to 4}\frac{8}{x-4}.
    \]
    We are only allowed to use this law if both limits exist.  Let's
    check each limit separately.
    \begin{align*}
      \displaystyle\lim_{x\to 4}\frac{2x}{x-4}=\frac{\lim_{x\to 4}2x}{\lim_{x\to 4}(x-4)}
    \end{align*}

and

    \begin{align*}
      \displaystyle\lim_{x\to 4}\frac{8}{x-4}=\displaystyle\frac{\lim_{x\to 4}8}{\lim_{x\to 4}(x-4)}
    \end{align*}
    
   We are only allowed to use this law if both limits exist. The limits in the numerators definitely
   exist. However, the denominator is equal to $0$ for both limits. Therefore, we cannot use the limit laws. 
   
   We can use algebra and simplify.
   
   \begin{align*}
   \displaystyle\lim_{x\to 4}\frac{2x-8}{x-4}&=\lim_{x\to 4}\frac{2(x-4)}{x-4}\\
   &=\lim_{x\to 4}2\\
   &=2
  \end{align*}
  Since the denominator is $0$, we cannot apply the Quotient Law.
  \end{feedback}
\end{question}

\begin{question}
  Can this limit be directly computed by limit laws?
  \[
  \displaystyle\lim_{x\to 0} \cot(x)\sin(x)
  \]
  \begin{multipleChoice}
    \choice{yes}
    \choice[correct]{no}
  \end{multipleChoice}
  \begin{feedback}
  If we are trying to use limit laws to compute this limit, we would
  have to use the Product Law to say that
  \[
  \displaystyle\lim_{x\to 0} \cot(x)\sin(x) =\lim_{x\to 0} \cot(x) \cdot \lim_{x\to 0}\sin(x).
  \]
  We are only allowed to use this law if both limits exist.  We know
  $\displaystyle\lim_{x\to 0} \sin(x) = 0$, but what about $\displaystyle\lim_{x\to 0}\cot(x)$?  We do
  not know how to find $\lim_{x\to 0}\cot(x)$ using limit laws because $0$
  is not in the domain of $\cot(x)$.
  \end{feedback}
  
  However, see what you can do with trigonometric identities. Try rewriting $\cot(x)$ as $\frac{\cos(x)}{\sin(x)}$
\end{question}


\begin{question}
  Can this limit be directly computed by limit laws?
  \[
  \displaystyle\lim_{x\to 0} \frac{\sin(x)}{1+x}
  \]
  \begin{multipleChoice}
    \choice[correct]{yes}
    \choice{no}
  \end{multipleChoice}
  \begin{question}
    Compute:
    \[
    \displaystyle\lim_{x\to 0} \frac{\sin(x)}{1+x}\begin{prompt} =\answer{0}\end{prompt}
    \]
    \begin{feedback}
      If we are trying to use limit laws to compute this limit, we
      would have to use the Quotient Law to say that
      \[
      \displaystyle\lim_{x\to 0} \frac{\sin(x)}{1+x} = \displaystyle\frac{\lim_{x\to
          0}\sin(x)}{\lim_{x\to 0}(1+x)}.
      \]
      We are only allowed to use this law if both limits exist and the
      denominator does not equal $0$.  Let's check each limit
      separately, starting with the denominator
      
      The limits in both the numerator and denominator exist and the
      limit in the denominator does not equal $0$, so we can use the
      Quotient Law.  We find:
      \[
        \displaystyle \frac{\lim_{x\to 0}\sin(x)}{\lim_{x\to 0}(1+x)}=\frac{0}{1}=0.
        \]
    \end{feedback}
  \end{question}
\end{question}


\begin{question}
  Can this limit be directly computed by limit laws?
  \[
  \displaystyle\lim_{x\to 0}(1+x)^{1/x}
  \]
  \begin{multipleChoice}
    \choice{yes}
    \choice[correct]{no}
  \end{multipleChoice}
  \begin{feedback}
  We do not have any limit laws for functions of the form $f(x)^{g(x)}$, so we cannot compute this limit.
  \end{feedback}
\end{question}

\end{document}
